@prefix : <http://www.semanticweb.org/david/ontologies/2/> .
@prefix owl: <http://www.w3.org/2002/07/owl#> .
@prefix rdf: <http://www.w3.org/1999/02/22-rdf-syntax-ns#> .
@prefix xml: <http://www.w3.org/XML/1998/namespace> .
@prefix xsd: <http://www.w3.org/2001/XMLSchema#> .
@prefix rdfs: <http://www.w3.org/2000/01/rdf-schema#> .
@prefix swrl: <http://www.w3.org/2003/11/swrl#> .
@prefix swrlb: <http://www.w3.org/2003/11/swrlb#> .
@prefix license: <http://creativecommons.org/licenses/by/4.0/> .
@prefix WinesOfSpain: <http://www.semanticweb.org/david/ontologies/2023/3/WinesOfSpain#> .
@base <http://www.semanticweb.org/david/ontologies/2/> .

<http://www.semanticweb.org/david/ontologies/2023/3/WinesOfSpain> rdf:type owl:Ontology ;
                                                                   rdfs:comment """Author: David Dorador
Date: 30/04/2023
Version: 1.0""" ;
                                                                   rdfs:label [ <http://creativecommons.org/ns#license> "http://creativecommons.org/licenses/by-sa/4.0/"
                                                                              ] ;
                                                                   rdfs:seeAlso "https://dbpedia.org/page/Wine" .

#################################################################
#    Annotation properties
#################################################################

###  http://creativecommons.org/ns#license
<http://creativecommons.org/ns#license> rdf:type owl:AnnotationProperty .


###  http://purl.org/dc/elements/1.1/rights
<http://purl.org/dc/elements/1.1/rights> rdf:type owl:AnnotationProperty .


###  http://purl.org/dc/terms/license
<http://purl.org/dc/terms/license> rdf:type owl:AnnotationProperty .


###  http://www.w3.org/2000/01/rdf-schema#sameAs
rdfs:sameAs rdf:type owl:AnnotationProperty .


#################################################################
#    Object Properties
#################################################################

###  http://www.semanticweb.org/david/ontologies/2023/3/WinesOfSpain#hasCharacteristic
WinesOfSpain:hasCharacteristic rdf:type owl:ObjectProperty ;
                               rdfs:domain WinesOfSpain:Wine ;
                               rdfs:range WinesOfSpain:WineCharacteristics ;
                               rdfs:comment "This property represents the relationship between a wine and its specific characteristics" .


###  http://www.semanticweb.org/david/ontologies/2023/3/WinesOfSpain#isAgedIn
WinesOfSpain:isAgedIn rdf:type owl:ObjectProperty ;
                      rdfs:domain WinesOfSpain:Wine ;
                      rdfs:range WinesOfSpain:AgingMethod ;
                      rdfs:comment "This property represents the relationship between a wine and the location where it has been aged, such as oak barrels, stainless steel tanks, or bottle" .


###  http://www.semanticweb.org/david/ontologies/2023/3/WinesOfSpain#isClassifiedAs
WinesOfSpain:isClassifiedAs rdf:type owl:ObjectProperty ;
                            rdfs:domain WinesOfSpain:Wine ;
                            rdfs:range WinesOfSpain:WineVariant ;
                            rdfs:comment "This property represents the relationship between a wine and its classification or category" .


###  http://www.semanticweb.org/david/ontologies/2023/3/WinesOfSpain#locatedIn
WinesOfSpain:locatedIn rdf:type owl:ObjectProperty ;
                       rdfs:domain WinesOfSpain:Winery ;
                       rdfs:range WinesOfSpain:Region ;
                       rdfs:comment "This property represents the relationship between a winery and its geographic location" .


###  http://www.semanticweb.org/david/ontologies/2023/3/WinesOfSpain#producedBy
WinesOfSpain:producedBy rdf:type owl:ObjectProperty ;
                        rdfs:domain WinesOfSpain:Wine ;
                        rdfs:range WinesOfSpain:Winery ;
                        rdfs:comment "This property represents the relationship between a wine and the winery that produces it" .


###  http://www.semanticweb.org/david/ontologies/2023/3/WinesOfSpain#producedIn
WinesOfSpain:producedIn rdf:type owl:ObjectProperty ;
                        rdfs:domain WinesOfSpain:Wine ;
                        rdfs:range WinesOfSpain:Region ;
                        rdfs:comment "This property represents the relationship between a wine and the location where it was produced" .


#################################################################
#    Data properties
#################################################################

###  http://www.semanticweb.org/david/ontologies/2023/3/WinesOfSpain#agingTime
WinesOfSpain:agingTime rdf:type owl:DatatypeProperty ,
                                owl:FunctionalProperty ;
                       rdfs:domain WinesOfSpain:Wine ;
                       rdfs:range xsd:integer ;
                       rdfs:comment "This property represents the amount of time in which a wine has been aged" .


###  http://www.semanticweb.org/david/ontologies/2023/3/WinesOfSpain#hasAlcohol
WinesOfSpain:hasAlcohol rdf:type owl:DatatypeProperty ;
                        rdfs:domain WinesOfSpain:Wine ;
                        rdfs:range xsd:float ;
                        rdfs:comment "This property represents the percentage of alcohol content in a bottle or unit of wine" .


###  http://www.semanticweb.org/david/ontologies/2023/3/WinesOfSpain#hasSugar
WinesOfSpain:hasSugar rdf:type owl:DatatypeProperty ;
                      rdfs:domain WinesOfSpain:Wine ;
                      rdfs:range xsd:float ;
                      rdfs:comment "This property represents the amount of sugar content in g/L" .


###  http://www.semanticweb.org/david/ontologies/2023/3/WinesOfSpain#hasYearFoundation
WinesOfSpain:hasYearFoundation rdf:type owl:DatatypeProperty ,
                                        owl:FunctionalProperty ;
                               rdfs:domain WinesOfSpain:Winery ;
                               rdfs:range xsd:integer ;
                               rdfs:comment "This property represents the year in which a winery was founded" .


###  http://www.semanticweb.org/david/ontologies/2023/3/WinesOfSpain#productionDay
WinesOfSpain:productionDay rdf:type owl:DatatypeProperty ,
                                    owl:FunctionalProperty ;
                           rdfs:domain WinesOfSpain:Wine ;
                           rdfs:range xsd:dateTime ;
                           rdfs:comment "This property represents the day or date on which a wine was produced" .


#################################################################
#    Classes
#################################################################

###  http://www.semanticweb.org/david/ontologies/2023/3/WinesOfSpain#Acidity
WinesOfSpain:Acidity rdf:type owl:Class ;
                     rdfs:subClassOf WinesOfSpain:WineCharacteristics ;
                     rdfs:comment "This class represents the acidity level of a wine, which is an important characteristic that affects its taste and aging potential" .


###  http://www.semanticweb.org/david/ontologies/2023/3/WinesOfSpain#AgingMethod
WinesOfSpain:AgingMethod rdf:type owl:Class ;
                         rdfs:subClassOf WinesOfSpain:WineCharacteristics ;
                         rdfs:comment "This class represents the amount of time that a wine has been aged in oak barrels or in the bottle, which can have a significant impact on its flavor, aroma, and texture" .


###  http://www.semanticweb.org/david/ontologies/2023/3/WinesOfSpain#Andalusia
WinesOfSpain:Andalusia rdf:type owl:Class ;
                       rdfs:subClassOf WinesOfSpain:Region ;
                       rdfs:comment "This class represents a region in southern Spain" .


###  http://www.semanticweb.org/david/ontologies/2023/3/WinesOfSpain#Average
WinesOfSpain:Average rdf:type owl:Class ;
                     rdfs:subClassOf WinesOfSpain:Price ;
                     rdfs:comment "This class represents a range of prices that is considered to be typical or average for wines" .


###  http://www.semanticweb.org/david/ontologies/2023/3/WinesOfSpain#Body
WinesOfSpain:Body rdf:type owl:Class ;
                  rdfs:subClassOf WinesOfSpain:WineCharacteristics ;
                  rdfs:comment "This class represents the weight and texture of a wine in the mouth, which is influenced by factors such as alcohol content, tannins, and sugar levels" .


###  http://www.semanticweb.org/david/ontologies/2023/3/WinesOfSpain#Catalonia
WinesOfSpain:Catalonia rdf:type owl:Class ;
                       rdfs:subClassOf WinesOfSpain:Region ;
                       rdfs:comment "This class represents a region in northeastern Spain" .


###  http://www.semanticweb.org/david/ontologies/2023/3/WinesOfSpain#Cheap
WinesOfSpain:Cheap rdf:type owl:Class ;
                   rdfs:subClassOf WinesOfSpain:Price ;
                   rdfs:comment "This class represents wines that are priced at or below the lower end of the price range" .


###  http://www.semanticweb.org/david/ontologies/2023/3/WinesOfSpain#DessertWine
WinesOfSpain:DessertWine rdf:type owl:Class ;
                         rdfs:subClassOf WinesOfSpain:WineVariant ;
                         owl:disjointWith WinesOfSpain:RedWine ,
                                          WinesOfSpain:RoséWine ,
                                          WinesOfSpain:SparklingWine ,
                                          WinesOfSpain:WhiteWine ;
                         rdfs:comment "This class represents a type of wine that is typically sweet, high in alcohol, and served in small quantities as a dessert accompaniment or after-dinner drink" ;
                         rdfs:sameAs "https://dbpedia.org/page/Dessert_wine" .


###  http://www.semanticweb.org/david/ontologies/2023/3/WinesOfSpain#Dry
WinesOfSpain:Dry rdf:type owl:Class ;
                 rdfs:subClassOf WinesOfSpain:Sugar ;
                 rdfs:comment "This class represents wines that contain very little or no residual sugar, and are characterized by their crisp, clean, and refreshing taste" .


###  http://www.semanticweb.org/david/ontologies/2023/3/WinesOfSpain#Exclusive
WinesOfSpain:Exclusive rdf:type owl:Class ;
                       rdfs:subClassOf WinesOfSpain:Price ;
                       rdfs:comment "This class represents wines that are priced at or above the upper end of the price range" .


###  http://www.semanticweb.org/david/ontologies/2023/3/WinesOfSpain#Expensive
WinesOfSpain:Expensive rdf:type owl:Class ;
                       rdfs:subClassOf WinesOfSpain:Price ;
                       rdfs:comment "This class represents wines that are priced significantly higher than the average or typical price" .


###  http://www.semanticweb.org/david/ontologies/2023/3/WinesOfSpain#Levante
WinesOfSpain:Levante rdf:type owl:Class ;
                     rdfs:subClassOf WinesOfSpain:Region ;
                     rdfs:comment "This class represents a region in eastern Spain" .


###  http://www.semanticweb.org/david/ontologies/2023/3/WinesOfSpain#North
WinesOfSpain:North rdf:type owl:Class ;
                   rdfs:subClassOf WinesOfSpain:Region ;
                   rdfs:comment "This class represents a broad geographic region in northern Spain" .


###  http://www.semanticweb.org/david/ontologies/2023/3/WinesOfSpain#Price
WinesOfSpain:Price rdf:type owl:Class ;
                   rdfs:subClassOf WinesOfSpain:WineCharacteristics ;
                   rdfs:comment "This class represents the cost of a bottle of wine, which can vary widely depending on factors such as the winery, region, vintage, and reputation" .


###  http://www.semanticweb.org/david/ontologies/2023/3/WinesOfSpain#RedWine
WinesOfSpain:RedWine rdf:type owl:Class ;
                     rdfs:subClassOf WinesOfSpain:WineVariant ;
                     owl:disjointWith WinesOfSpain:RoséWine ,
                                      WinesOfSpain:SparklingWine ,
                                      WinesOfSpain:WhiteWine ;
                     rdfs:comment "This class represents a type of wine that is made from red or black grapes and is typically medium- to full-bodied, with flavors and aromas that vary depending on the grape variety, region, and aging process" ;
                     rdfs:sameAs "http://dbpedia.org/page/Red_wine" .


###  http://www.semanticweb.org/david/ontologies/2023/3/WinesOfSpain#Region
WinesOfSpain:Region rdf:type owl:Class ;
                    rdfs:comment "This class represents a geographic area or location that is known for producing wines" .


###  http://www.semanticweb.org/david/ontologies/2023/3/WinesOfSpain#Rioja
WinesOfSpain:Rioja rdf:type owl:Class ;
                   rdfs:subClassOf WinesOfSpain:Region ;
                   rdfs:comment "This class represents a specific wine region in northern Spain" .


###  http://www.semanticweb.org/david/ontologies/2023/3/WinesOfSpain#RoséWine
WinesOfSpain:RoséWine rdf:type owl:Class ;
                      rdfs:subClassOf WinesOfSpain:WineVariant ;
                      owl:disjointWith WinesOfSpain:SparklingWine ,
                                       WinesOfSpain:WhiteWine ;
                      rdfs:comment "This class represents a type of wine that is made from red or black grapes but is only briefly allowed to come into contact with the grape skins, resulting in a pink or salmon color and a lighter, more delicate flavor profile" ;
                      rdfs:sameAs "https://dbpedia.org/page/Ros%C3%A9" .


###  http://www.semanticweb.org/david/ontologies/2023/3/WinesOfSpain#SemiDry
WinesOfSpain:SemiDry rdf:type owl:Class ;
                     rdfs:subClassOf WinesOfSpain:Sugar ;
                     rdfs:comment "This class represents wines that contain a moderate amount of residual sugar, and are characterized by their balance of sweetness and acidity" .


###  http://www.semanticweb.org/david/ontologies/2023/3/WinesOfSpain#SemiSweet
WinesOfSpain:SemiSweet rdf:type owl:Class ;
                       rdfs:subClassOf WinesOfSpain:Sugar ;
                       rdfs:comment "This class represents wines that contain a higher amount of residual sugar than SemiDry wines, and are characterized by their fruity, floral, or honeyed notes" .


###  http://www.semanticweb.org/david/ontologies/2023/3/WinesOfSpain#SparklingWine
WinesOfSpain:SparklingWine rdf:type owl:Class ;
                           rdfs:subClassOf WinesOfSpain:WineVariant ;
                           owl:disjointWith WinesOfSpain:WhiteWine ;
                           rdfs:comment "This class represents a type of wine that contains significant levels of carbon dioxide, resulting in bubbles or effervescence, and is typically associated with celebratory occasions or special events" ;
                           rdfs:sameAs "https://dbpedia.org/page/Sparkling_wine" .


###  http://www.semanticweb.org/david/ontologies/2023/3/WinesOfSpain#Sugar
WinesOfSpain:Sugar rdf:type owl:Class ;
                   rdfs:subClassOf WinesOfSpain:WineCharacteristics ;
                   rdfs:comment "This class represents the amount of residual sugar in a wine, which can affect its sweetness and overall balance of flavors" ;
                   rdfs:sameAs "https://dbpedia.org/page/Sugars_in_wine" .


###  http://www.semanticweb.org/david/ontologies/2023/3/WinesOfSpain#Sweet
WinesOfSpain:Sweet rdf:type owl:Class ;
                   rdfs:subClassOf WinesOfSpain:Sugar ;
                   rdfs:comment "This class represents wines that contain a significant amount of residual sugar, and are characterized by their intense sweetness and rich, complex flavors" .


###  http://www.semanticweb.org/david/ontologies/2023/3/WinesOfSpain#WhiteWine
WinesOfSpain:WhiteWine rdf:type owl:Class ;
                       rdfs:subClassOf WinesOfSpain:WineVariant ;
                       rdfs:comment "This class represents a type of wine that is made from white grapes or from red grapes with the skins removed, and is typically light-bodied, crisp, and refreshing" ;
                       rdfs:sameAs "https://dbpedia.org/page/White_wine" .


###  http://www.semanticweb.org/david/ontologies/2023/3/WinesOfSpain#Wine
WinesOfSpain:Wine rdf:type owl:Class ;
                  owl:equivalentClass [ rdf:type owl:Restriction ;
                                        owl:onProperty WinesOfSpain:productionDay ;
                                        owl:qualifiedCardinality "1"^^xsd:nonNegativeInteger ;
                                        owl:onDataRange xsd:dateTime
                                      ] ;
                  rdfs:comment "This class represents a type of alcoholic beverage that is produced by fermenting grapes" .


###  http://www.semanticweb.org/david/ontologies/2023/3/WinesOfSpain#WineCharacteristics
WinesOfSpain:WineCharacteristics rdf:type owl:Class ;
                                 rdfs:comment "Characteristics of the wine" .


###  http://www.semanticweb.org/david/ontologies/2023/3/WinesOfSpain#WineVariant
WinesOfSpain:WineVariant rdf:type owl:Class ;
                         rdfs:comment "This class represents a specific type or style of wine that is distinguished by its grape variety, geographic origin, production methods, or other unique characteristics" .


###  http://www.semanticweb.org/david/ontologies/2023/3/WinesOfSpain#Winery
WinesOfSpain:Winery rdf:type owl:Class ;
                    rdfs:subClassOf [ rdf:type owl:Restriction ;
                                      owl:onProperty WinesOfSpain:hasYearFoundation ;
                                      owl:qualifiedCardinality "1"^^xsd:nonNegativeInteger ;
                                      owl:onDataRange xsd:integer
                                    ] ;
                    rdfs:comment "This class represents a wine-producing company or facility that grows grapes, produces wine, and markets it under its own brand name" .


#################################################################
#    Individuals
#################################################################

###  http://www.semanticweb.org/david/ontologies/2023/3/WinesOfSpain#Barrel
WinesOfSpain:Barrel rdf:type owl:NamedIndividual ,
                             WinesOfSpain:AgingMethod ;
                    rdfs:sameAs "https://dbpedia.org/page/Barrel" .


###  http://www.semanticweb.org/david/ontologies/2023/3/WinesOfSpain#Bodega_Jose_Pariente
WinesOfSpain:Bodega_Jose_Pariente rdf:type owl:NamedIndividual ,
                                           WinesOfSpain:Winery ;
                                  WinesOfSpain:locatedIn WinesOfSpain:La_Seca ;
                                  WinesOfSpain:hasYearFoundation 1960 .


###  http://www.semanticweb.org/david/ontologies/2023/3/WinesOfSpain#Bottle
WinesOfSpain:Bottle rdf:type owl:NamedIndividual ,
                             WinesOfSpain:AgingMethod .


###  http://www.semanticweb.org/david/ontologies/2023/3/WinesOfSpain#Corpinnat
WinesOfSpain:Corpinnat rdf:type owl:NamedIndividual ,
                                WinesOfSpain:Catalonia .


###  http://www.semanticweb.org/david/ontologies/2023/3/WinesOfSpain#Garnacha
WinesOfSpain:Garnacha rdf:type owl:NamedIndividual ,
                               WinesOfSpain:RedWine ;
                      rdfs:sameAs "https://dbpedia.org/page/Grenache" .


###  http://www.semanticweb.org/david/ontologies/2023/3/WinesOfSpain#Jose_Pariente_Verdejo
WinesOfSpain:Jose_Pariente_Verdejo rdf:type owl:NamedIndividual ,
                                            WinesOfSpain:Wine ;
                                   WinesOfSpain:isAgedIn WinesOfSpain:Bottle ;
                                   WinesOfSpain:isClassifiedAs WinesOfSpain:Verdejo ;
                                   WinesOfSpain:producedBy WinesOfSpain:Bodega_Jose_Pariente ;
                                   WinesOfSpain:producedIn WinesOfSpain:La_Seca ;
                                   WinesOfSpain:agingTime 100 ;
                                   WinesOfSpain:hasAlcohol "13.2"^^xsd:float ;
                                   WinesOfSpain:hasSugar "12.4"^^xsd:float ;
                                   WinesOfSpain:productionDay "2022-08-01T10:00:00"^^xsd:dateTime .


###  http://www.semanticweb.org/david/ontologies/2023/3/WinesOfSpain#La_Montesa
WinesOfSpain:La_Montesa rdf:type owl:NamedIndividual ,
                                 WinesOfSpain:Wine ;
                        WinesOfSpain:isAgedIn WinesOfSpain:Barrel ;
                        WinesOfSpain:isClassifiedAs WinesOfSpain:Garnacha ;
                        WinesOfSpain:producedBy WinesOfSpain:Palacios_Redondo ;
                        WinesOfSpain:producedIn WinesOfSpain:Rioja_Oriental ;
                        WinesOfSpain:agingTime 367 ;
                        WinesOfSpain:hasAlcohol "14.5"^^xsd:float ;
                        WinesOfSpain:hasSugar "30.6"^^xsd:float ;
                        WinesOfSpain:productionDay "2019-08-17T08:00:00"^^xsd:dateTime .


###  http://www.semanticweb.org/david/ontologies/2023/3/WinesOfSpain#La_Seca
WinesOfSpain:La_Seca rdf:type owl:NamedIndividual ,
                              WinesOfSpain:North .


###  http://www.semanticweb.org/david/ontologies/2023/3/WinesOfSpain#Llopart
WinesOfSpain:Llopart rdf:type owl:NamedIndividual ;
                     WinesOfSpain:locatedIn WinesOfSpain:Corpinnat ;
                     WinesOfSpain:hasYearFoundation 1980 .


###  http://www.semanticweb.org/david/ontologies/2023/3/WinesOfSpain#Llopart_Microcosmos
WinesOfSpain:Llopart_Microcosmos rdf:type owl:NamedIndividual ,
                                          WinesOfSpain:Wine ;
                                 WinesOfSpain:isAgedIn WinesOfSpain:Barrel ;
                                 WinesOfSpain:isClassifiedAs WinesOfSpain:Pinot_Noir ;
                                 WinesOfSpain:producedBy WinesOfSpain:Llopart ;
                                 WinesOfSpain:producedIn WinesOfSpain:Corpinnat ;
                                 WinesOfSpain:agingTime 720 ;
                                 WinesOfSpain:hasAlcohol "11.9"^^xsd:float ;
                                 WinesOfSpain:hasSugar "40.0"^^xsd:float ;
                                 WinesOfSpain:productionDay "2019-08-10T09:00:00"^^xsd:dateTime .


###  http://www.semanticweb.org/david/ontologies/2023/3/WinesOfSpain#Palacios_Redondo
WinesOfSpain:Palacios_Redondo rdf:type owl:NamedIndividual ,
                                       WinesOfSpain:Winery .


###  http://www.semanticweb.org/david/ontologies/2023/3/WinesOfSpain#Pinot_Noir
WinesOfSpain:Pinot_Noir rdf:type owl:NamedIndividual ,
                                 WinesOfSpain:SparklingWine ;
                        rdfs:sameAs "https://es.dbpedia.org/page/Pinot_noir" .


###  http://www.semanticweb.org/david/ontologies/2023/3/WinesOfSpain#Rioja_Oriental
WinesOfSpain:Rioja_Oriental rdf:type owl:NamedIndividual ,
                                     WinesOfSpain:Rioja .


###  http://www.semanticweb.org/david/ontologies/2023/3/WinesOfSpain#Verdejo
WinesOfSpain:Verdejo rdf:type owl:NamedIndividual ,
                              WinesOfSpain:WhiteWine .


#################################################################
#    Rules
#################################################################

<urn:swrl:var#w> rdf:type swrl:Variable .

<urn:swrl:var#s> rdf:type swrl:Variable .

[ rdf:type swrl:Imp ;
   swrl:body [ rdf:type swrl:AtomList ;
               rdf:first [ rdf:type swrl:ClassAtom ;
                           swrl:classPredicate WinesOfSpain:Wine ;
                           swrl:argument1 <urn:swrl:var#w>
                         ] ;
               rdf:rest [ rdf:type swrl:AtomList ;
                          rdf:first [ rdf:type swrl:BuiltinAtom ;
                                      swrl:builtin swrlb:greaterThanOrEqual ;
                                      swrl:arguments [ rdf:type rdf:List ;
                                                       rdf:first <urn:swrl:var#s> ;
                                                       rdf:rest [ rdf:type rdf:List ;
                                                                  rdf:first 45 ;
                                                                  rdf:rest rdf:nil
                                                                ]
                                                     ]
                                    ] ;
                          rdf:rest [ rdf:type swrl:AtomList ;
                                     rdf:first [ rdf:type swrl:DatavaluedPropertyAtom ;
                                                 swrl:propertyPredicate WinesOfSpain:hasSugar ;
                                                 swrl:argument1 <urn:swrl:var#w> ;
                                                 swrl:argument2 <urn:swrl:var#s>
                                               ] ;
                                     rdf:rest rdf:nil
                                   ]
                        ]
             ] ;
   swrl:head [ rdf:type swrl:AtomList ;
               rdf:first [ rdf:type swrl:ClassAtom ;
                           swrl:classPredicate WinesOfSpain:Sweet ;
                           swrl:argument1 <urn:swrl:var#w>
                         ] ;
               rdf:rest rdf:nil
             ]
 ] .

[ rdf:type swrl:Imp ;
   swrl:body [ rdf:type swrl:AtomList ;
               rdf:first [ rdf:type swrl:ClassAtom ;
                           swrl:classPredicate WinesOfSpain:Wine ;
                           swrl:argument1 <urn:swrl:var#w>
                         ] ;
               rdf:rest [ rdf:type swrl:AtomList ;
                          rdf:first [ rdf:type swrl:BuiltinAtom ;
                                      swrl:builtin swrlb:greaterThanOrEqual ;
                                      swrl:arguments [ rdf:type rdf:List ;
                                                       rdf:first <urn:swrl:var#s> ;
                                                       rdf:rest [ rdf:type rdf:List ;
                                                                  rdf:first 9 ;
                                                                  rdf:rest rdf:nil
                                                                ]
                                                     ]
                                    ] ;
                          rdf:rest [ rdf:type swrl:AtomList ;
                                     rdf:first [ rdf:type swrl:BuiltinAtom ;
                                                 swrl:builtin swrlb:lessThan ;
                                                 swrl:arguments [ rdf:type rdf:List ;
                                                                  rdf:first <urn:swrl:var#s> ;
                                                                  rdf:rest [ rdf:type rdf:List ;
                                                                             rdf:first 18 ;
                                                                             rdf:rest rdf:nil
                                                                           ]
                                                                ]
                                               ] ;
                                     rdf:rest [ rdf:type swrl:AtomList ;
                                                rdf:first [ rdf:type swrl:DatavaluedPropertyAtom ;
                                                            swrl:propertyPredicate WinesOfSpain:hasSugar ;
                                                            swrl:argument1 <urn:swrl:var#w> ;
                                                            swrl:argument2 <urn:swrl:var#s>
                                                          ] ;
                                                rdf:rest rdf:nil
                                              ]
                                   ]
                        ]
             ] ;
   swrl:head [ rdf:type swrl:AtomList ;
               rdf:first [ rdf:type swrl:ClassAtom ;
                           swrl:classPredicate WinesOfSpain:SemiDry ;
                           swrl:argument1 <urn:swrl:var#w>
                         ] ;
               rdf:rest rdf:nil
             ]
 ] .

[ rdf:type swrl:Imp ;
   swrl:body [ rdf:type swrl:AtomList ;
               rdf:first [ rdf:type swrl:ClassAtom ;
                           swrl:classPredicate WinesOfSpain:Wine ;
                           swrl:argument1 <urn:swrl:var#w>
                         ] ;
               rdf:rest [ rdf:type swrl:AtomList ;
                          rdf:first [ rdf:type swrl:BuiltinAtom ;
                                      swrl:builtin swrlb:greaterThanOrEqual ;
                                      swrl:arguments [ rdf:type rdf:List ;
                                                       rdf:first <urn:swrl:var#s> ;
                                                       rdf:rest [ rdf:type rdf:List ;
                                                                  rdf:first 18 ;
                                                                  rdf:rest rdf:nil
                                                                ]
                                                     ]
                                    ] ;
                          rdf:rest [ rdf:type swrl:AtomList ;
                                     rdf:first [ rdf:type swrl:BuiltinAtom ;
                                                 swrl:builtin swrlb:lessThan ;
                                                 swrl:arguments [ rdf:type rdf:List ;
                                                                  rdf:first <urn:swrl:var#s> ;
                                                                  rdf:rest [ rdf:type rdf:List ;
                                                                             rdf:first 45 ;
                                                                             rdf:rest rdf:nil
                                                                           ]
                                                                ]
                                               ] ;
                                     rdf:rest [ rdf:type swrl:AtomList ;
                                                rdf:first [ rdf:type swrl:DatavaluedPropertyAtom ;
                                                            swrl:propertyPredicate WinesOfSpain:hasSugar ;
                                                            swrl:argument1 <urn:swrl:var#w> ;
                                                            swrl:argument2 <urn:swrl:var#s>
                                                          ] ;
                                                rdf:rest rdf:nil
                                              ]
                                   ]
                        ]
             ] ;
   swrl:head [ rdf:type swrl:AtomList ;
               rdf:first [ rdf:type swrl:ClassAtom ;
                           swrl:classPredicate WinesOfSpain:SemiSweet ;
                           swrl:argument1 <urn:swrl:var#w>
                         ] ;
               rdf:rest rdf:nil
             ]
 ] .

[ rdf:type swrl:Imp ;
   swrl:body [ rdf:type swrl:AtomList ;
               rdf:first [ rdf:type swrl:ClassAtom ;
                           swrl:classPredicate WinesOfSpain:Wine ;
                           swrl:argument1 <urn:swrl:var#w>
                         ] ;
               rdf:rest [ rdf:type swrl:AtomList ;
                          rdf:first [ rdf:type swrl:BuiltinAtom ;
                                      swrl:builtin swrlb:lessThan ;
                                      swrl:arguments [ rdf:type rdf:List ;
                                                       rdf:first <urn:swrl:var#s> ;
                                                       rdf:rest [ rdf:type rdf:List ;
                                                                  rdf:first 9 ;
                                                                  rdf:rest rdf:nil
                                                                ]
                                                     ]
                                    ] ;
                          rdf:rest [ rdf:type swrl:AtomList ;
                                     rdf:first [ rdf:type swrl:DatavaluedPropertyAtom ;
                                                 swrl:propertyPredicate WinesOfSpain:hasSugar ;
                                                 swrl:argument1 <urn:swrl:var#w> ;
                                                 swrl:argument2 <urn:swrl:var#s>
                                               ] ;
                                     rdf:rest rdf:nil
                                   ]
                        ]
             ] ;
   swrl:head [ rdf:type swrl:AtomList ;
               rdf:first [ rdf:type swrl:ClassAtom ;
                           swrl:classPredicate WinesOfSpain:Dry ;
                           swrl:argument1 <urn:swrl:var#w>
                         ] ;
               rdf:rest rdf:nil
             ]
 ] .

###  Generated by the OWL API (version 4.5.25.2023-02-15T19:15:49Z) https://github.com/owlcs/owlapi
